tests/coq/hashmap_on_disk/HashmapMain_Funs.v
@@ -14,20 +14,28 @@ Module HashmapMain_Funs.
 Definition hashmap_hash_key_fwd (k : usize) : result usize := Return k.
 
 (** [hashmap_main::hashmap::HashMap::{0}::allocate_slots] *)
-Fixpoint hashmap_hash_map_allocate_slots_fwd
-  (T : Type) (n : nat) (slots : vec (Hashmap_list_t T)) (n0 : usize) :
+Fixpoint hashmap_hash_map_allocate_slots_loop_fwd
+  (T : Type) (n : nat) (v : vec (Hashmap_list_t T)) (n0 : usize) :
   result (vec (Hashmap_list_t T))
   :=
   match n with
   | O => Fail_ OutOfFuel
   | S n1 =>
-    if n0 s= 0%usize
-    then Return slots
-    else (
-      slots0 <- vec_push_back (Hashmap_list_t T) slots HashmapListNil;
-      i <- usize_sub n0 1%usize;
-      hashmap_hash_map_allocate_slots_fwd T n1 slots0 i)
+    if n0 s> 0%usize
+    then (
+      slots <- vec_push_back (Hashmap_list_t T) v HashmapListNil;
+      n2 <- usize_sub n0 1%usize;
+      hashmap_hash_map_allocate_slots_loop_fwd T n1 slots n2)
+    else Return v
   end
+.
+
+(** [hashmap_main::hashmap::HashMap::{0}::allocate_slots] *)
+Definition hashmap_hash_map_allocate_slots_fwd
+  (T : Type) (n : nat) (slots : vec (Hashmap_list_t T)) (n0 : usize) :
+  result (vec (Hashmap_list_t T))
+  :=
+  hashmap_hash_map_allocate_slots_loop_fwd T n slots n0
 .
 
 (** [hashmap_main::hashmap::HashMap::{0}::new_with_capacity] *)
@@ -51,21 +59,29 @@ Definition hashmap_hash_map_new_fwd
 .
 
 (** [hashmap_main::hashmap::HashMap::{0}::clear_slots] *)
-Fixpoint hashmap_hash_map_clear_slots_fwd_back
-  (T : Type) (n : nat) (slots : vec (Hashmap_list_t T)) (i : usize) :
+Fixpoint hashmap_hash_map_clear_slots_loop_fwd_back
+  (T : Type) (n : nat) (v : vec (Hashmap_list_t T)) (i : usize) :
   result (vec (Hashmap_list_t T))
   :=
   match n with
   | O => Fail_ OutOfFuel
   | S n0 =>
-    let i0 := vec_len (Hashmap_list_t T) slots in
+    let i0 := vec_len (Hashmap_list_t T) v in
     if i s< i0
     then (
-      slots0 <- vec_index_mut_back (Hashmap_list_t T) slots i HashmapListNil;
       i1 <- usize_add i 1%usize;
-      hashmap_hash_map_clear_slots_fwd_back T n0 slots0 i1)
-    else Return slots
+      slots <- vec_index_mut_back (Hashmap_list_t T) v i HashmapListNil;
+      hashmap_hash_map_clear_slots_loop_fwd_back T n0 slots i1)
+    else Return v
   end
+.
+
+(** [hashmap_main::hashmap::HashMap::{0}::clear_slots] *)
+Definition hashmap_hash_map_clear_slots_fwd_back
+  (T : Type) (n : nat) (slots : vec (Hashmap_list_t T)) :
+  result (vec (Hashmap_list_t T))
+  :=
+  hashmap_hash_map_clear_slots_loop_fwd_back T n slots (0%usize)
 .
 
 (** [hashmap_main::hashmap::HashMap::{0}::clear] *)
@@ -73,9 +89,7 @@ Definition hashmap_hash_map_clear_fwd_back
   (T : Type) (n : nat) (self : Hashmap_hash_map_t T) :
   result (Hashmap_hash_map_t T)
   :=
-  v <-
-    hashmap_hash_map_clear_slots_fwd_back T n self.(Hashmap_hash_map_slots)
-      (0%usize);
+  v <- hashmap_hash_map_clear_slots_fwd_back T n self.(Hashmap_hash_map_slots);
   Return (mkHashmap_hash_map_t (0%usize)
     self.(Hashmap_hash_map_max_load_factor) self.(Hashmap_hash_map_max_load) v)
 .
@@ -87,7 +101,7 @@ Definition hashmap_hash_map_len_fwd
 .
 
 (** [hashmap_main::hashmap::HashMap::{0}::insert_in_list] *)
-Fixpoint hashmap_hash_map_insert_in_list_fwd
+Fixpoint hashmap_hash_map_insert_in_list_loop_fwd
   (T : Type) (n : nat) (key : usize) (value : T) (ls : Hashmap_list_t T) :
   result bool
   :=
@@ -95,17 +109,25 @@ Fixpoint hashmap_hash_map_insert_in_list_fwd
   | O => Fail_ OutOfFuel
   | S n0 =>
     match ls with
-    | HashmapListCons ckey cvalue ls0 =>
+    | HashmapListCons ckey cvalue tl =>
       if ckey s= key
       then Return false
-      else hashmap_hash_map_insert_in_list_fwd T n0 key value ls0
+      else hashmap_hash_map_insert_in_list_loop_fwd T n0 key value tl
     | HashmapListNil => Return true
     end
   end
 .
 
 (** [hashmap_main::hashmap::HashMap::{0}::insert_in_list] *)
-Fixpoint hashmap_hash_map_insert_in_list_back
+Definition hashmap_hash_map_insert_in_list_fwd
+  (T : Type) (n : nat) (key : usize) (value : T) (ls : Hashmap_list_t T) :
+  result bool
+  :=
+  hashmap_hash_map_insert_in_list_loop_fwd T n key value ls
+.
+
+(** [hashmap_main::hashmap::HashMap::{0}::insert_in_list] *)
+Fixpoint hashmap_hash_map_insert_in_list_loop_back
   (T : Type) (n : nat) (key : usize) (value : T) (ls : Hashmap_list_t T) :
   result (Hashmap_list_t T)
   :=
@@ -113,16 +135,24 @@ Fixpoint hashmap_hash_map_insert_in_list_back
   | O => Fail_ OutOfFuel
   | S n0 =>
     match ls with
-    | HashmapListCons ckey cvalue ls0 =>
+    | HashmapListCons ckey cvalue tl =>
       if ckey s= key
-      then Return (HashmapListCons ckey value ls0)
+      then Return (HashmapListCons ckey value tl)
       else (
-        ls1 <- hashmap_hash_map_insert_in_list_back T n0 key value ls0;
-        Return (HashmapListCons ckey cvalue ls1))
+        l <- hashmap_hash_map_insert_in_list_loop_back T n0 key value tl;
+        Return (HashmapListCons ckey cvalue l))
     | HashmapListNil =>
       let l := HashmapListNil in Return (HashmapListCons key value l)
     end
   end
+.
+
+(** [hashmap_main::hashmap::HashMap::{0}::insert_in_list] *)
+Definition hashmap_hash_map_insert_in_list_back
+  (T : Type) (n : nat) (key : usize) (value : T) (ls : Hashmap_list_t T) :
+  result (Hashmap_list_t T)
+  :=
+  hashmap_hash_map_insert_in_list_loop_back T n key value ls
 .
 
 (** [hashmap_main::hashmap::HashMap::{0}::insert_no_resize] *)
@@ -161,9 +191,8 @@ Definition core_num_u32_max_body : result u32 := Return (4294967295%u32).
 Definition core_num_u32_max_c : u32 := core_num_u32_max_body%global.
 
 (** [hashmap_main::hashmap::HashMap::{0}::move_elements_from_list] *)
-Fixpoint hashmap_hash_map_move_elements_from_list_fwd_back
-  (T : Type) (n : nat) (ntable : Hashmap_hash_map_t T) (ls : Hashmap_list_t T)
-  :
+Fixpoint hashmap_hash_map_move_elements_from_list_loop_fwd_back
+  (T : Type) (n : nat) (hm : Hashmap_hash_map_t T) (ls : Hashmap_list_t T) :
   result (Hashmap_hash_map_t T)
   :=
   match n with
@@ -171,35 +200,52 @@ Fixpoint hashmap_hash_map_move_elements_from_list_fwd_back
   | S n0 =>
     match ls with
     | HashmapListCons k v tl =>
-      ntable0 <- hashmap_hash_map_insert_no_resize_fwd_back T n0 ntable k v;
-      hashmap_hash_map_move_elements_from_list_fwd_back T n0 ntable0 tl
-    | HashmapListNil => Return ntable
+      ntable <- hashmap_hash_map_insert_no_resize_fwd_back T n0 hm k v;
+      hashmap_hash_map_move_elements_from_list_loop_fwd_back T n0 ntable tl
+    | HashmapListNil => Return hm
     end
   end
 .
 
+(** [hashmap_main::hashmap::HashMap::{0}::move_elements_from_list] *)
+Definition hashmap_hash_map_move_elements_from_list_fwd_back
+  (T : Type) (n : nat) (ntable : Hashmap_hash_map_t T) (ls : Hashmap_list_t T)
+  :
+  result (Hashmap_hash_map_t T)
+  :=
+  hashmap_hash_map_move_elements_from_list_loop_fwd_back T n ntable ls
+.
+
 (** [hashmap_main::hashmap::HashMap::{0}::move_elements] *)
-Fixpoint hashmap_hash_map_move_elements_fwd_back
-  (T : Type) (n : nat) (ntable : Hashmap_hash_map_t T)
-  (slots : vec (Hashmap_list_t T)) (i : usize) :
+Fixpoint hashmap_hash_map_move_elements_loop_fwd_back
+  (T : Type) (n : nat) (hm : Hashmap_hash_map_t T) (v : vec (Hashmap_list_t T))
+  (i : usize) :
   result ((Hashmap_hash_map_t T) * (vec (Hashmap_list_t T)))
   :=
   match n with
   | O => Fail_ OutOfFuel
   | S n0 =>
-    let i0 := vec_len (Hashmap_list_t T) slots in
+    let i0 := vec_len (Hashmap_list_t T) v in
     if i s< i0
     then (
-      l <- vec_index_mut_fwd (Hashmap_list_t T) slots i;
+      l <- vec_index_mut_fwd (Hashmap_list_t T) v i;
       let ls := mem_replace_fwd (Hashmap_list_t T) l HashmapListNil in
-      ntable0 <-
-        hashmap_hash_map_move_elements_from_list_fwd_back T n0 ntable ls;
-      let l0 := mem_replace_back (Hashmap_list_t T) l HashmapListNil in
-      slots0 <- vec_index_mut_back (Hashmap_list_t T) slots i l0;
+      ntable <- hashmap_hash_map_move_elements_from_list_fwd_back T n0 hm ls;
       i1 <- usize_add i 1%usize;
-      hashmap_hash_map_move_elements_fwd_back T n0 ntable0 slots0 i1)
-    else Return (ntable, slots)
+      let l0 := mem_replace_back (Hashmap_list_t T) l HashmapListNil in
+      slots <- vec_index_mut_back (Hashmap_list_t T) v i l0;
+      hashmap_hash_map_move_elements_loop_fwd_back T n0 ntable slots i1)
+    else Return (hm, v)
   end
+.
+
+(** [hashmap_main::hashmap::HashMap::{0}::move_elements] *)
+Definition hashmap_hash_map_move_elements_fwd_back
+  (T : Type) (n : nat) (ntable : Hashmap_hash_map_t T)
+  (slots : vec (Hashmap_list_t T)) (i : usize) :
+  result ((Hashmap_hash_map_t T) * (vec (Hashmap_list_t T)))
+  :=
+  hashmap_hash_map_move_elements_loop_fwd_back T n ntable slots i
 .
 
 (** [hashmap_main::hashmap::HashMap::{0}::try_resize] *)
@@ -241,19 +287,25 @@ Definition hashmap_hash_map_insert_fwd_back
 .
 
 (** [hashmap_main::hashmap::HashMap::{0}::contains_key_in_list] *)
-Fixpoint hashmap_hash_map_contains_key_in_list_fwd
-  (T : Type) (n : nat) (key : usize) (ls : Hashmap_list_t T) : result bool :=
+Fixpoint hashmap_hash_map_contains_key_in_list_loop_fwd
+  (T : Type) (n : nat) (i : usize) (ls : Hashmap_list_t T) : result bool :=
   match n with
   | O => Fail_ OutOfFuel
   | S n0 =>
     match ls with
-    | HashmapListCons ckey t ls0 =>
-      if ckey s= key
+    | HashmapListCons ckey t tl =>
+      if ckey s= i
       then Return true
-      else hashmap_hash_map_contains_key_in_list_fwd T n0 key ls0
+      else hashmap_hash_map_contains_key_in_list_loop_fwd T n0 i tl
     | HashmapListNil => Return false
     end
   end
+.
+
+(** [hashmap_main::hashmap::HashMap::{0}::contains_key_in_list] *)
+Definition hashmap_hash_map_contains_key_in_list_fwd
+  (T : Type) (n : nat) (key : usize) (ls : Hashmap_list_t T) : result bool :=
+  hashmap_hash_map_contains_key_in_list_loop_fwd T n key ls
 .
 
 (** [hashmap_main::hashmap::HashMap::{0}::contains_key] *)
@@ -269,19 +321,25 @@ Definition hashmap_hash_map_contains_key_fwd
 .
 
 (** [hashmap_main::hashmap::HashMap::{0}::get_in_list] *)
-Fixpoint hashmap_hash_map_get_in_list_fwd
-  (T : Type) (n : nat) (key : usize) (ls : Hashmap_list_t T) : result T :=
+Fixpoint hashmap_hash_map_get_in_list_loop_fwd
+  (T : Type) (n : nat) (i : usize) (ls : Hashmap_list_t T) : result T :=
   match n with
   | O => Fail_ OutOfFuel
   | S n0 =>
     match ls with
-    | HashmapListCons ckey cvalue ls0 =>
-      if ckey s= key
+    | HashmapListCons ckey cvalue tl =>
+      if ckey s= i
       then Return cvalue
-      else hashmap_hash_map_get_in_list_fwd T n0 key ls0
+      else hashmap_hash_map_get_in_list_loop_fwd T n0 i tl
     | HashmapListNil => Fail_ Failure
     end
   end
+.
+
+(** [hashmap_main::hashmap::HashMap::{0}::get_in_list] *)
+Definition hashmap_hash_map_get_in_list_fwd
+  (T : Type) (n : nat) (key : usize) (ls : Hashmap_list_t T) : result T :=
+  hashmap_hash_map_get_in_list_loop_fwd T n key ls
 .
 
 (** [hashmap_main::hashmap::HashMap::{0}::get] *)
@@ -297,39 +355,53 @@ Definition hashmap_hash_map_get_fwd
 .
 
 (** [hashmap_main::hashmap::HashMap::{0}::get_mut_in_list] *)
-Fixpoint hashmap_hash_map_get_mut_in_list_fwd
-  (T : Type) (n : nat) (key : usize) (ls : Hashmap_list_t T) : result T :=
+Fixpoint hashmap_hash_map_get_mut_in_list_loop_fwd
+  (T : Type) (n : nat) (i : usize) (ls : Hashmap_list_t T) : result T :=
   match n with
   | O => Fail_ OutOfFuel
   | S n0 =>
     match ls with
-    | HashmapListCons ckey cvalue ls0 =>
-      if ckey s= key
+    | HashmapListCons ckey cvalue tl =>
+      if ckey s= i
       then Return cvalue
-      else hashmap_hash_map_get_mut_in_list_fwd T n0 key ls0
+      else hashmap_hash_map_get_mut_in_list_loop_fwd T n0 i tl
     | HashmapListNil => Fail_ Failure
     end
   end
 .
 
 (** [hashmap_main::hashmap::HashMap::{0}::get_mut_in_list] *)
-Fixpoint hashmap_hash_map_get_mut_in_list_back
-  (T : Type) (n : nat) (key : usize) (ls : Hashmap_list_t T) (ret : T) :
+Definition hashmap_hash_map_get_mut_in_list_fwd
+  (T : Type) (n : nat) (ls : Hashmap_list_t T) (key : usize) : result T :=
+  hashmap_hash_map_get_mut_in_list_loop_fwd T n key ls
+.
+
+(** [hashmap_main::hashmap::HashMap::{0}::get_mut_in_list] *)
+Fixpoint hashmap_hash_map_get_mut_in_list_loop_back
+  (T : Type) (n : nat) (i : usize) (ls : Hashmap_list_t T) (ret : T) :
   result (Hashmap_list_t T)
   :=
   match n with
   | O => Fail_ OutOfFuel
   | S n0 =>
     match ls with
-    | HashmapListCons ckey cvalue ls0 =>
-      if ckey s= key
-      then Return (HashmapListCons ckey ret ls0)
+    | HashmapListCons ckey cvalue tl =>
+      if ckey s= i
+      then Return (HashmapListCons ckey ret tl)
       else (
-        ls1 <- hashmap_hash_map_get_mut_in_list_back T n0 key ls0 ret;
-        Return (HashmapListCons ckey cvalue ls1))
+        l <- hashmap_hash_map_get_mut_in_list_loop_back T n0 i tl ret;
+        Return (HashmapListCons ckey cvalue l))
     | HashmapListNil => Fail_ Failure
     end
   end
+.
+
+(** [hashmap_main::hashmap::HashMap::{0}::get_mut_in_list] *)
+Definition hashmap_hash_map_get_mut_in_list_back
+  (T : Type) (n : nat) (ls : Hashmap_list_t T) (key : usize) (ret : T) :
+  result (Hashmap_list_t T)
+  :=
+  hashmap_hash_map_get_mut_in_list_loop_back T n key ls ret
 .
 
 (** [hashmap_main::hashmap::HashMap::{0}::get_mut] *)
@@ -342,7 +414,7 @@ Definition hashmap_hash_map_get_mut_fwd
   hash_mod <- usize_rem hash i;
   l <-
     vec_index_mut_fwd (Hashmap_list_t T) self.(Hashmap_hash_map_slots) hash_mod;
-  hashmap_hash_map_get_mut_in_list_fwd T n key l
+  hashmap_hash_map_get_mut_in_list_fwd T n l key
 .
 
 (** [hashmap_main::hashmap::HashMap::{0}::get_mut] *)
@@ -355,7 +427,7 @@ Definition hashmap_hash_map_get_mut_back
   hash_mod <- usize_rem hash i;
   l <-
     vec_index_mut_fwd (Hashmap_list_t T) self.(Hashmap_hash_map_slots) hash_mod;
-  l0 <- hashmap_hash_map_get_mut_in_list_back T n key l ret;
+  l0 <- hashmap_hash_map_get_mut_in_list_back T n l key ret;
   v <-
     vec_index_mut_back (Hashmap_list_t T) self.(Hashmap_hash_map_slots)
       hash_mod l0;
@@ -364,8 +436,8 @@ Definition hashmap_hash_map_get_mut_back
 .
 
 (** [hashmap_main::hashmap::HashMap::{0}::remove_from_list] *)
-Fixpoint hashmap_hash_map_remove_from_list_fwd
-  (T : Type) (n : nat) (key : usize) (ls : Hashmap_list_t T) :
+Fixpoint hashmap_hash_map_remove_from_list_loop_fwd
+  (T : Type) (n : nat) (i : usize) (ls : Hashmap_list_t T) :
   result (option T)
   :=
   match n with
@@ -373,24 +445,32 @@ Fixpoint hashmap_hash_map_remove_from_list_fwd
   | S n0 =>
     match ls with
     | HashmapListCons ckey t tl =>
-      if ckey s= key
+      if ckey s= i
       then
         let mv_ls :=
           mem_replace_fwd (Hashmap_list_t T) (HashmapListCons ckey t tl)
             HashmapListNil in
         match mv_ls with
-        | HashmapListCons i cvalue tl0 => Return (Some cvalue)
+        | HashmapListCons i0 cvalue tl0 => Return (Some cvalue)
         | HashmapListNil => Fail_ Failure
         end
-      else hashmap_hash_map_remove_from_list_fwd T n0 key tl
+      else hashmap_hash_map_remove_from_list_loop_fwd T n0 i tl
     | HashmapListNil => Return None
     end
   end
 .
 
 (** [hashmap_main::hashmap::HashMap::{0}::remove_from_list] *)
-Fixpoint hashmap_hash_map_remove_from_list_back
+Definition hashmap_hash_map_remove_from_list_fwd
   (T : Type) (n : nat) (key : usize) (ls : Hashmap_list_t T) :
+  result (option T)
+  :=
+  hashmap_hash_map_remove_from_list_loop_fwd T n key ls
+.
+
+(** [hashmap_main::hashmap::HashMap::{0}::remove_from_list] *)
+Fixpoint hashmap_hash_map_remove_from_list_loop_back
+  (T : Type) (n : nat) (i : usize) (ls : Hashmap_list_t T) :
   result (Hashmap_list_t T)
   :=
   match n with
@@ -398,21 +478,29 @@ Fixpoint hashmap_hash_map_remove_from_list_back
   | S n0 =>
     match ls with
     | HashmapListCons ckey t tl =>
-      if ckey s= key
+      if ckey s= i
       then
         let mv_ls :=
           mem_replace_fwd (Hashmap_list_t T) (HashmapListCons ckey t tl)
             HashmapListNil in
         match mv_ls with
-        | HashmapListCons i cvalue tl0 => Return tl0
+        | HashmapListCons i0 cvalue tl0 => Return tl0
         | HashmapListNil => Fail_ Failure
         end
       else (
-        tl0 <- hashmap_hash_map_remove_from_list_back T n0 key tl;
-        Return (HashmapListCons ckey t tl0))
+        l <- hashmap_hash_map_remove_from_list_loop_back T n0 i tl;
+        Return (HashmapListCons ckey t l))
     | HashmapListNil => Return HashmapListNil
     end
   end
+.
+
+(** [hashmap_main::hashmap::HashMap::{0}::remove_from_list] *)
+Definition hashmap_hash_map_remove_from_list_back
+  (T : Type) (n : nat) (key : usize) (ls : Hashmap_list_t T) :
+  result (Hashmap_list_t T)
+  :=
+  hashmap_hash_map_remove_from_list_loop_back T n key ls
 .
 
 (** [hashmap_main::hashmap::HashMap::{0}::remove] *)
@@ -429,8 +517,7 @@ Definition hashmap_hash_map_remove_fwd
   match x with
   | None => Return None
   | Some x0 =>
-    i0 <- usize_sub self.(Hashmap_hash_map_num_entries) 1%usize;
-    let _ := i0 in
+    _ <- usize_sub self.(Hashmap_hash_map_num_entries) 1%usize;
     Return (Some x0)
   end
 .
