tests/fstar/hashmap_on_disk/HashmapMain.Clauses.Template.fst
@@ -9,13 +9,13 @@ open HashmapMain.Types
 (** [hashmap_main::hashmap::HashMap::{0}::allocate_slots]: decreases clause *)
 unfold
 let hashmap_hash_map_allocate_slots_decreases (t : Type0)
-  (slots : vec (hashmap_list_t t)) (n : usize) : nat =
+  (v : vec (hashmap_list_t t)) (n : usize) : nat =
   admit ()
 
 (** [hashmap_main::hashmap::HashMap::{0}::clear_slots]: decreases clause *)
 unfold
 let hashmap_hash_map_clear_slots_decreases (t : Type0)
-  (slots : vec (hashmap_list_t t)) (i : usize) : nat =
+  (v : vec (hashmap_list_t t)) (i : usize) : nat =
   admit ()
 
 (** [hashmap_main::hashmap::HashMap::{0}::insert_in_list]: decreases clause *)
@@ -31,37 +31,36 @@ let core_num_u32_max_c : u32 = eval_global core_num_u32_max_body
 (** [hashmap_main::hashmap::HashMap::{0}::move_elements_from_list]: decreases clause *)
 unfold
 let hashmap_hash_map_move_elements_from_list_decreases (t : Type0)
-  (ntable : hashmap_hash_map_t t) (ls : hashmap_list_t t) : nat =
+  (hm : hashmap_hash_map_t t) (ls : hashmap_list_t t) : nat =
   admit ()
 
 (** [hashmap_main::hashmap::HashMap::{0}::move_elements]: decreases clause *)
 unfold
 let hashmap_hash_map_move_elements_decreases (t : Type0)
-  (ntable : hashmap_hash_map_t t) (slots : vec (hashmap_list_t t)) (i : usize)
-  : nat =
+  (hm : hashmap_hash_map_t t) (v : vec (hashmap_list_t t)) (i : usize) : nat =
   admit ()
 
 (** [hashmap_main::hashmap::HashMap::{0}::contains_key_in_list]: decreases clause *)
 unfold
-let hashmap_hash_map_contains_key_in_list_decreases (t : Type0) (key : usize)
+let hashmap_hash_map_contains_key_in_list_decreases (t : Type0) (i : usize)
   (ls : hashmap_list_t t) : nat =
   admit ()
 
 (** [hashmap_main::hashmap::HashMap::{0}::get_in_list]: decreases clause *)
 unfold
-let hashmap_hash_map_get_in_list_decreases (t : Type0) (key : usize)
+let hashmap_hash_map_get_in_list_decreases (t : Type0) (i : usize)
   (ls : hashmap_list_t t) : nat =
   admit ()
 
 (** [hashmap_main::hashmap::HashMap::{0}::get_mut_in_list]: decreases clause *)
 unfold
-let hashmap_hash_map_get_mut_in_list_decreases (t : Type0) (key : usize)
+let hashmap_hash_map_get_mut_in_list_decreases (t : Type0) (i : usize)
   (ls : hashmap_list_t t) : nat =
   admit ()
 
 (** [hashmap_main::hashmap::HashMap::{0}::remove_from_list]: decreases clause *)
 unfold
-let hashmap_hash_map_remove_from_list_decreases (t : Type0) (key : usize)
+let hashmap_hash_map_remove_from_list_decreases (t : Type0) (i : usize)
   (ls : hashmap_list_t t) : nat =
   admit ()
 
